Added top-level certification function.

checker/coq/log.v
@@ -7,11 +7,13 @@ Require Import domain.
 Require Import model.
 Require Import map.
 Require Import resolution.
+Require Import Recdef.
 Module ZMapProperties := FMapFacts.WProperties(ZMaps).
 
 Definition clause_map := zmap clause.
 Definition cst_map := zmap cst.
 
+                            
 Inductive step :=
   | Intro : Z -> clause -> step
   | Hint : Z -> step
@@ -29,6 +31,27 @@ Inductive status :=
 Definition eval_cstmap cs theta :=
   forall (id : Z) (c : cst),
     ZMaps.MapsTo id c cs -> eval_cst c theta.
+
+Fixpoint cst_map_of_csts cs :=
+  match cs with
+  | nil => ZMaps.empty cst
+  | cons (k, c) cs' =>
+      ZMaps.add k c (cst_map_of_csts cs')
+  end.
+Lemma cst_map_if_csts : forall (cs : list (Z * cst)) (theta : asg),
+  eval_csts cs theta -> eval_cstmap (cst_map_of_csts cs) theta.
+Proof.
+  induction cs.
+
+  unfold eval_cstmap, cst_map_of_csts; intros; now apply ZMapProperties.F.empty_mapsto_iff in H0.
+
+  unfold eval_csts, eval_cstmap; fold eval_csts; fold eval_cstmap; destruct a; simpl in *; intros.
+  destruct H as [Hc Hcs].
+  apply ZMapProperties.F.add_mapsto_iff in H0.
+  destruct H0 as [He | Hd]; [destruct He as [Hz Hc0] | destruct Hd as [Hd Hmap]].
+    rewrite <- Hc0; assumption.
+    apply IHcs in Hcs; unfold eval_cstmap in Hcs; now apply Hcs with (id := id).
+Qed.
 
 Definition state_csts (s : state) :=
   match s with
@@ -54,6 +77,18 @@ Definition state_valid (s : state) :=
         eval_cstmap cs theta -> eval_clause cl theta
   end.
   
+Definition empty_state (m : model) :=
+  match m with
+  | (bs, cs) => (cst_map_of_csts cs, ZMaps.empty clause, (-1))
+  end.
+
+Lemma empty_state_valid : forall m, state_valid (empty_state m).
+Proof.
+  unfold state_valid, empty_state; intros; destruct m; simpl in *.
+  intros.
+  now apply ZMapProperties.F.empty_mapsto_iff in H.  
+Qed.
+
 Definition clause_map_add (cs : clause_map) (id : Z) (cl : clause) := ZMaps.add id cl cs.
 
 Definition clause_map_del (cs : clause_map) (id : Z) := ZMaps.remove id cs.
@@ -218,4 +253,154 @@ Proof.
     now apply set_hint_valid.
     now apply del_clause_valid.
     now apply apply_resolution_valid.
+Qed.
+
+Fixpoint apply_step_list (s : state) (ds : list step) :=
+  match ds with
+  | nil => s
+  | cons d ds' => apply_step_list (apply_step s d) ds'
+  end.
+       
+Theorem apply_step_list_valid : forall (ds : list step) (s : state),
+  state_valid s -> state_valid (apply_step_list s ds).
+Proof.
+  induction ds.
+    intros; now unfold apply_step_list.
+
+    unfold apply_step_list; fold apply_step_list. 
+    intros; apply IHds.
+    now apply apply_step_valid.
+Qed.
+
+CoInductive steps :=
+  | Fin : steps
+  | Steps : step -> steps -> steps.
+
+Function apply_steps (s : state) (lim : Z) (ds : steps) { measure Zabs_nat lim } :=
+  if Z_leb lim (0%Z) then
+    s 
+  else
+    match ds with
+    | Fin => s
+    | Steps d ds' =>
+       apply_steps (apply_step s d) (Zpred lim) ds'
+    end.
+  intros.
+  apply Z_leb_false_iff_notle in teq.
+  apply Zabs_nat_lt; omega.
+Defined.
+
+Definition apply_steps_validP s (lim : Z) (ds : steps) s' :=
+  state_valid s -> state_valid s'.
+
+Theorem apply_steps_valid : forall (s : state) (lim : Z) (ds : steps),
+  state_valid s -> state_valid (apply_steps s lim ds).
+Proof.
+  assert (Hi := apply_steps_ind apply_steps_validP).
+  unfold apply_steps_validP in *.
+  intros; apply Hi.
+    trivial.
+    trivial.
+
+    intros.
+    apply H0.    
+    now apply apply_step_valid.
+    assumption.
+Qed.
+
+Fixpoint contains_false (cs : list (Z * clause)) :=
+  match cs with
+  | nil => false
+  | cons (_, c) cs' =>
+    match c with
+    | nil => true
+    | _ => contains_false cs'
+    end
+  end.
+
+Lemma contains_false_1 : forall cs, contains_false cs = true -> exists k, List.In (k, nil) cs.
+Proof.
+  induction cs.
+    unfold contains_false; discriminate.
+
+    unfold contains_false; fold contains_false.
+    destruct a; destruct c; simpl in *; intros.
+      exists z; now left.
+
+    apply IHcs in H.
+    elim H.
+    intros.
+    exists x.
+    now right.
+Qed.
+
+Lemma contains_false_unsat : forall (cs : clause_map),
+  contains_false (ZMaps.elements cs) = true -> forall theta, ~ eval_clmap cs theta.
+Proof.
+  intros.
+  apply contains_false_1 in H.
+  intro Hcs.
+  unfold eval_clmap in Hcs.
+  elim H; intros.
+  assert (eval_clause nil theta).
+  apply Hcs with (id := x).
+  rewrite ZMapProperties.F.elements_mapsto_iff.
+  apply SetoidList.In_InA with (eqA := ZMaps.eq_key_elt (elt := clause)) in H0; try assumption.
+  apply ZMapProperties.eqke_equiv.
+  now unfold eval_clause in H1.
+Qed.
+
+Definition state_unsat (s : state) :=
+  match s with
+  | (_, cs, _) => contains_false (ZMaps.elements cs)
+  end.
+
+Lemma state_unsat_valid : forall s, state_unsat s = true -> state_valid s -> forall theta, ~ eval_cstmap (state_csts s) theta.
+Proof.
+  intros s.
+  unfold state_unsat, state_valid.
+  destruct s; destruct p; simpl.
+  intros.
+  intro; unfold eval_cstmap.
+  apply contains_false_1 in H.
+  elim H; intros.
+  apply SetoidList.In_InA with (eqA := ZMaps.eq_key_elt (elt := clause)) in H2.
+  apply ZMapProperties.F.elements_mapsto_iff in H2.
+  apply H0 with (theta := theta) in H2.
+  now unfold eval_clause in H2.
+  assumption.
+  apply ZMapProperties.eqke_equiv.
+Qed.
+
+Lemma state_csts_const : forall s lim ss, state_csts s = state_csts (apply_steps s lim ss).
+Proof.
+  set (I s (_ : Z) (_ : steps) s' := state_csts s = state_csts s').
+  apply apply_steps_ind with (P := I); unfold I; clear I; intros;
+    unfold state_csts in *; destruct s; destruct p; simpl in *; try congruence.
+  rewrite <- H.  
+  unfold apply_step; try unfold apply_inference; simpl; try congruence.
+  destruct d; simpl; try congruence.
+  destruct (ZMaps.find (elt := cst) z z0); simpl; try congruence.
+  destruct (check_cst c0 c); try congruence.
+Qed.
+  
+Definition certify_unsat (m : model) (lim : Z) (s : steps) :=
+  state_unsat (apply_steps (empty_state m) lim s). 
+Theorem certify_unsat_valid : forall m lim s,
+  certify_unsat m lim s = true -> model_unsat m.
+Proof.
+  intros m lim s.
+  unfold certify_unsat, model_unsat.
+  intros.
+  assert (Hs0 := empty_state_valid m).
+  apply (apply_steps_valid (empty_state m) lim s) in Hs0.
+  intros Hem.
+  unfold eval_model in Hem; destruct Hem as [Hb Hcs].
+  apply state_unsat_valid with (theta := theta) in H.
+  rewrite <- state_csts_const in H.
+  clear Hs0.
+  destruct m; unfold empty_state, state_csts in *; simpl in *.
+  apply cst_map_if_csts in Hcs.
+  contradiction.
+  assumption.
 Qed.
